wip: bignum32

code/bignum/Hacl.Spec.Bignum.Exponentiation.fst
@@ -9,7 +9,7 @@ open Lib.LoopCombinators
 open Hacl.Spec.Bignum.Definitions
 open Hacl.Spec.Bignum
 open Hacl.Spec.Bignum.Montgomery
-open Hacl.Spec.Bignum.ModInv64
+open Hacl.Spec.Bignum.ModInvLimb
 
 module BL = Hacl.Spec.Exponentiation.Lemmas
 module M = Hacl.Spec.Montgomery.Lemmas
@@ -17,24 +17,25 @@ module M = Hacl.Spec.Montgomery.Lemmas
 
 #reset-options "--z3rlimit 50 --fuel 0 --ifuel 0"
 
-let check_mod_exp #nLen n a bBits b =
+let check_mod_exp #t #nLen n a bBits b =
+  let pbits = bits t in
   let m0 = check_modulus n in
   let m1 = bn_is_zero_mask b in
   bn_is_zero_mask_lemma b;
   assert (if v m1 = 0 then bn_v b > 0 else bn_v b = 0);
-  assert (v m1 = 0 \/ v m1 = ones_v U64);
+  assert (v m1 = 0 \/ v m1 = ones_v t);
   let m1' = lognot m1 in
   lognot_lemma m1;
   assert (if v m1' = 0 then bn_v b = 0 else bn_v b > 0);
 
-  bn_eval_bound b (blocks bBits 64);
+  bn_eval_bound b (blocks bBits pbits);
   let m2 =
-    if bBits < 64 * blocks bBits 64 then begin
+    if bBits < pbits * blocks bBits pbits then begin
       bn_lt_pow2_mask_lemma b bBits;
       bn_lt_pow2_mask b bBits end
     else begin
-      Math.Lemmas.pow2_le_compat bBits (64 * blocks bBits 64);
-      ones U64 SEC end in
+      Math.Lemmas.pow2_le_compat bBits (pbits * blocks bBits pbits);
+      ones t SEC end in
   assert (if v m2 = 0 then pow2 bBits <= bn_v b else bn_v b < pow2 bBits);
 
   let m3 = bn_lt_mask a n in
@@ -51,207 +52,226 @@ let check_mod_exp #nLen n a bBits b =
   r
 
 
-val bn_mod_exp_f:
-    #nLen:size_pos{nLen + nLen <= max_size_t}
-  -> n:lbignum nLen
-  -> mu:uint64
-  -> bBits:size_pos
-  -> bLen:size_nat{bLen == blocks bBits 64}
-  -> b:lbignum bLen
-  -> i:nat{i < bBits}
-  -> aM_accM: tuple2 (lbignum nLen) (lbignum nLen) ->
-  tuple2 (lbignum nLen) (lbignum nLen)
+val unsafe_bn_is_ith_bit_set:
+    #t:limb_t
+  -> #len:size_nat
+  -> b:lbignum t len
+  -> i:size_nat{i / bits t < len} ->
+  bool
 
-let bn_mod_exp_f #nLen n mu bBits bLen b i (aM, accM) =
-  let is_bit_set = FStar.UInt64.(Lib.RawIntTypes.u64_to_UInt64 (bn_get_ith_bit #bLen b i) =^ 1uL) in
+let unsafe_bn_is_ith_bit_set #t #len b i =
+  match t with
+  | U32 -> FStar.UInt32.(Lib.RawIntTypes.u32_to_UInt32 (bn_get_ith_bit b i) =^ 1ul)
+  | U64 -> FStar.UInt64.(Lib.RawIntTypes.u64_to_UInt64 (bn_get_ith_bit b i) =^ 1uL)
+
+
+val bn_mod_exp_f:
+    #t:limb_t
+  -> #nLen:size_pos{nLen + nLen <= max_size_t}
+  -> n:lbignum t nLen
+  -> mu:limb t
+  -> bBits:size_pos
+  -> bLen:size_nat{bLen == blocks bBits (bits t)}
+  -> b:lbignum t bLen
+  -> i:nat{i < bBits}
+  -> aM_accM: tuple2 (lbignum t nLen) (lbignum t nLen) ->
+  tuple2 (lbignum t nLen) (lbignum t nLen)
+
+let bn_mod_exp_f #t #nLen n mu bBits bLen b i (aM, accM) =
+  let is_bit_set = unsafe_bn_is_ith_bit_set b i in
   let accM = if is_bit_set then mont_mul n mu aM accM else accM in // acc = (acc * a) % n
   let aM = mont_sqr n mu aM in // a = (a * a) % n
   (aM, accM)
 
 
 val bn_mod_exp_mont:
-    nLen:size_pos{128 * nLen <= max_size_t}
-  -> n:lbignum nLen
-  -> a:lbignum nLen
-  -> acc:lbignum nLen
+    #t:limb_t
+  -> nLen:size_pos{2 * bits t * nLen <= max_size_t}
+  -> n:lbignum t nLen
+  -> a:lbignum t nLen
+  -> acc:lbignum t nLen
   -> bBits:size_pos
-  -> b:lbignum (blocks bBits 64)
-  -> r2:lbignum nLen ->
-  lbignum nLen
+  -> b:lbignum t (blocks bBits (bits t))
+  -> r2:lbignum t nLen ->
+  lbignum t nLen
 
-let bn_mod_exp_mont nLen n a acc bBits b r2 =
-  let bLen = blocks bBits 64 in
-  let mu = mod_inv_u64 n.[0] in
+let bn_mod_exp_mont #t nLen n a acc bBits b r2 =
+  let bLen = blocks bBits (bits t) in
+  let mu = mod_inv_limb n.[0] in
 
   let aM = to_mont n mu r2 a in
   let accM = to_mont n mu r2 acc in
-  let (aM, accM) = repeati bBits (bn_mod_exp_f #nLen n mu bBits bLen b) (aM, accM) in
+  let (aM, accM) = repeati bBits (bn_mod_exp_f n mu bBits bLen b) (aM, accM) in
   from_mont n mu accM
 
 
-let bn_mod_exp_precompr2 nLen n a bBits b r2 =
-  let acc = bn_from_uint nLen (u64 1) in
+let bn_mod_exp_precompr2 #t nLen n a bBits b r2 =
+  let acc = bn_from_uint nLen (uint #t 1) in
   bn_mod_exp_mont nLen n a acc bBits b r2
 
 
 val bn_mod_exp_f_lemma:
-    #nLen:size_pos{nLen + nLen <= max_size_t}
-  -> n:lbignum nLen
-  -> mu:uint64
+    #t:limb_t
+  -> #nLen:size_pos{nLen + nLen <= max_size_t}
+  -> n:lbignum t nLen
+  -> mu:limb t
   -> bBits:size_pos
-  -> bLen:size_nat{bLen == blocks bBits 64}
-  -> b:lbignum bLen
+  -> bLen:size_nat{bLen == blocks bBits (bits t)}
+  -> b:lbignum t bLen
   -> i:nat{i < bBits}
-  -> aM_accM0: tuple2 (lbignum nLen) (lbignum nLen) -> Lemma
+  -> aM_accM0: tuple2 (lbignum t nLen) (lbignum t nLen) -> Lemma
   (requires
    (let (aM0, accM0) = aM_accM0 in
-    (1 + (bn_v n % pow2 64) * v mu) % pow2 64 == 0 /\
+    (1 + (bn_v n % pow2 (bits t)) * v mu) % pow2 (bits t) == 0 /\
     bn_v n % 2 = 1 /\ 1 < bn_v n /\
     0 < bn_v b /\ bn_v b < pow2 bBits /\
     bn_v aM0 < bn_v n /\ bn_v accM0 < bn_v n))
   (ensures
    (let (aM0, accM0) = aM_accM0 in
-    let (aM1, accM1) = bn_mod_exp_f #nLen n mu bBits bLen b i aM_accM0 in
-    let (aM2, accM2) = BL.mod_exp_mont_f_ll nLen (bn_v n) (v mu) bBits (bn_v b) i (bn_v aM0, bn_v accM0) in
+    let (aM1, accM1) = bn_mod_exp_f n mu bBits bLen b i aM_accM0 in
+    let (aM2, accM2) = BL.mod_exp_mont_f_ll (bits t) nLen (bn_v n) (v mu) bBits (bn_v b) i (bn_v aM0, bn_v accM0) in
     bn_v aM1 == aM2 /\ bn_v accM1 == accM2 /\
     bn_v aM1 < bn_v n /\ bn_v accM1 < bn_v n))
 
-let bn_mod_exp_f_lemma #nLen n mu bBits bLen b i (aM0, accM0) =
-  let (aM1, accM1) = bn_mod_exp_f #nLen n mu bBits bLen b i (aM0, accM0) in
-  let (aM2, accM2) = BL.mod_exp_mont_f_ll nLen (bn_v n) (v mu) bBits (bn_v b) i (bn_v aM0, bn_v accM0) in
-  mont_sqr_lemma #nLen n mu aM0;
+let bn_mod_exp_f_lemma #t #nLen n mu bBits bLen b i (aM0, accM0) =
+  let (aM1, accM1) = bn_mod_exp_f n mu bBits bLen b i (aM0, accM0) in
+  let (aM2, accM2) = BL.mod_exp_mont_f_ll (bits t) nLen (bn_v n) (v mu) bBits (bn_v b) i (bn_v aM0, bn_v accM0) in
+  mont_sqr_lemma n mu aM0;
   assert (bn_v aM1 == aM2);
-  bn_get_ith_bit_lemma #bLen b i;
-  if (bn_v b / pow2 i % 2 = 1) then mont_mul_lemma #nLen n mu aM0 accM0;
+  bn_get_ith_bit_lemma b i;
+  if (bn_v b / pow2 i % 2 = 1) then mont_mul_lemma n mu aM0 accM0;
   assert (bn_v accM1 == accM2)
 
 
 val bn_mod_exp_mont_loop_lemma:
-    #nLen:size_pos{nLen + nLen <= max_size_t}
-  -> n:lbignum nLen
-  -> mu:uint64
+    #t:limb_t
+  -> #nLen:size_pos{nLen + nLen <= max_size_t}
+  -> n:lbignum t nLen
+  -> mu:limb t
   -> bBits:size_pos
-  -> bLen:size_nat{bLen == blocks bBits 64}
-  -> b:lbignum bLen
+  -> bLen:size_nat{bLen == blocks bBits (bits t)}
+  -> b:lbignum t bLen
   -> i:size_nat{i <= bBits}
-  -> aM_accM0: tuple2 (lbignum nLen) (lbignum nLen) -> Lemma
+  -> aM_accM0: tuple2 (lbignum t nLen) (lbignum t nLen) -> Lemma
   (requires
    (let (aM0, accM0) = aM_accM0 in
-    (1 + (bn_v n % pow2 64) * v mu) % pow2 64 == 0 /\
+    (1 + (bn_v n % pow2 (bits t)) * v mu) % pow2 (bits t) == 0 /\
     bn_v n % 2 = 1 /\ 1 < bn_v n /\
     0 < bn_v b /\ bn_v b < pow2 bBits /\
     bn_v aM0 < bn_v n /\ bn_v accM0 < bn_v n))
   (ensures
    (let (aM0, accM0) = aM_accM0 in
-    let (aM1, accM1) = repeati i (bn_mod_exp_f #nLen n mu bBits bLen b) (aM0, accM0) in
-    let (aM2, accM2) = repeati i (BL.mod_exp_mont_f_ll nLen (bn_v n) (v mu) bBits (bn_v b)) (bn_v aM0, bn_v accM0) in
+    let (aM1, accM1) = repeati i (bn_mod_exp_f n mu bBits bLen b) (aM0, accM0) in
+    let (aM2, accM2) = repeati i (BL.mod_exp_mont_f_ll (bits t) nLen (bn_v n) (v mu) bBits (bn_v b)) (bn_v aM0, bn_v accM0) in
     bn_v aM1 == aM2 /\ bn_v accM1 == accM2 /\
     bn_v aM1 < bn_v n /\ bn_v accM1 < bn_v n))
 
-let rec bn_mod_exp_mont_loop_lemma #nLen n mu bBits bLen b i (aM0, accM0) =
-  let (aM1, accM1) = repeati i (bn_mod_exp_f #nLen n mu bBits bLen b) (aM0, accM0) in
-  let (aM2, accM2) = repeati i (BL.mod_exp_mont_f_ll nLen (bn_v n) (v mu) bBits (bn_v b)) (bn_v aM0, bn_v accM0) in
+let rec bn_mod_exp_mont_loop_lemma #t #nLen n mu bBits bLen b i (aM0, accM0) =
+  let (aM1, accM1) = repeati i (bn_mod_exp_f n mu bBits bLen b) (aM0, accM0) in
+  let (aM2, accM2) = repeati i (BL.mod_exp_mont_f_ll (bits t) nLen (bn_v n) (v mu) bBits (bn_v b)) (bn_v aM0, bn_v accM0) in
 
   if i = 0 then begin
-    eq_repeati0 i (bn_mod_exp_f #nLen n mu bBits bLen b) (aM0, accM0);
-    eq_repeati0 i (BL.mod_exp_mont_f_ll nLen (bn_v n) (v mu) bBits (bn_v b)) (bn_v aM0, bn_v accM0);
+    eq_repeati0 i (bn_mod_exp_f n mu bBits bLen b) (aM0, accM0);
+    eq_repeati0 i (BL.mod_exp_mont_f_ll (bits t) nLen (bn_v n) (v mu) bBits (bn_v b)) (bn_v aM0, bn_v accM0);
     () end
   else begin
-    unfold_repeati i (bn_mod_exp_f #nLen n mu bBits bLen b) (aM0, accM0) (i - 1);
-    unfold_repeati i (BL.mod_exp_mont_f_ll nLen (bn_v n) (v mu) bBits (bn_v b)) (bn_v aM0, bn_v accM0) (i - 1);
-    let (aM3, accM3) = repeati (i - 1) (bn_mod_exp_f #nLen n mu bBits bLen b) (aM0, accM0) in
-    let (aM4, accM4) = repeati (i - 1) (BL.mod_exp_mont_f_ll nLen (bn_v n) (v mu) bBits (bn_v b)) (bn_v aM0, bn_v accM0) in
-    assert ((aM1, accM1) == bn_mod_exp_f #nLen n mu bBits bLen b (i - 1) (aM3, accM3));
-    assert ((aM2, accM2) == BL.mod_exp_mont_f_ll nLen (bn_v n) (v mu) bBits (bn_v b) (i - 1) (aM4, accM4));
-    bn_mod_exp_mont_loop_lemma #nLen n mu bBits bLen b (i - 1) (aM0, accM0);
+    unfold_repeati i (bn_mod_exp_f n mu bBits bLen b) (aM0, accM0) (i - 1);
+    unfold_repeati i (BL.mod_exp_mont_f_ll (bits t) nLen (bn_v n) (v mu) bBits (bn_v b)) (bn_v aM0, bn_v accM0) (i - 1);
+    let (aM3, accM3) = repeati (i - 1) (bn_mod_exp_f n mu bBits bLen b) (aM0, accM0) in
+    let (aM4, accM4) = repeati (i - 1) (BL.mod_exp_mont_f_ll (bits t) nLen (bn_v n) (v mu) bBits (bn_v b)) (bn_v aM0, bn_v accM0) in
+    assert ((aM1, accM1) == bn_mod_exp_f n mu bBits bLen b (i - 1) (aM3, accM3));
+    assert ((aM2, accM2) == BL.mod_exp_mont_f_ll (bits t) nLen (bn_v n) (v mu) bBits (bn_v b) (i - 1) (aM4, accM4));
+    bn_mod_exp_mont_loop_lemma n mu bBits bLen b (i - 1) (aM0, accM0);
     assert (bn_v aM3 == aM4 /\ bn_v accM3 == accM4);
-    bn_mod_exp_f_lemma #nLen n mu bBits bLen b (i - 1) (aM3, accM3);
+    bn_mod_exp_f_lemma n mu bBits bLen b (i - 1) (aM3, accM3);
     () end
 
 
 val bn_mod_exp_mont_lemma_aux:
-    nLen:size_pos{128 * nLen <= max_size_t}
-  -> n:lbignum nLen
-  -> a:lbignum nLen
+    #t:limb_t
+  -> nLen:size_pos{2 * bits t * nLen <= max_size_t}
+  -> n:lbignum t nLen
+  -> a:lbignum t nLen
   -> bBits:size_pos
-  -> b:lbignum (blocks bBits 64)
-  -> r2:lbignum nLen -> Lemma
+  -> b:lbignum t (blocks bBits (bits t))
+  -> r2:lbignum t nLen -> Lemma
   (requires
     bn_v n % 2 = 1 /\ 1 < bn_v n /\
     0 < bn_v b /\ bn_v b < pow2 bBits /\ bn_v a < bn_v n /\
-    bn_v r2 == pow2 (128 * nLen) % bn_v n)
+    bn_v r2 == pow2 (2 * bits t * nLen) % bn_v n)
   (ensures
-   (let mu = mod_inv_u64 n.[0] in
+   (let mu = mod_inv_limb n.[0] in
     let res1 = bn_mod_exp_precompr2 nLen n a bBits b r2 in
-    let res2 = BL.mod_exp_mont_ll nLen (bn_v n) (v mu) (bn_v a) bBits (bn_v b) in
+    let res2 = BL.mod_exp_mont_ll (bits t) nLen (bn_v n) (v mu) (bn_v a) bBits (bn_v b) in
     bn_v res1 == res2 /\ bn_v res1 < bn_v n))
 
-let bn_mod_exp_mont_lemma_aux nLen n a bBits b r2 =
-  let bLen = blocks bBits 64 in
+let bn_mod_exp_mont_lemma_aux #t nLen n a bBits b r2 =
+  let bLen = blocks bBits (bits t) in
 
-  let acc = bn_from_uint nLen (u64 1) in
-  bn_from_uint_lemma nLen (u64 1);
+  let acc = bn_from_uint nLen (uint #t 1) in
+  bn_from_uint_lemma nLen (uint #t 1);
   assert (bn_v acc == 1);
 
-  let mu = mod_inv_u64 n.[0] in
+  let mu = mod_inv_limb n.[0] in
   bn_eval_index n 0;
-  assert (bn_v n % pow2 64 == v n.[0]);
-  Math.Lemmas.pow2_modulo_modulo_lemma_1 (bn_v n) 2 64;
+  assert (bn_v n % pow2 (bits t) == v n.[0]);
+  Math.Lemmas.pow2_modulo_modulo_lemma_1 (bn_v n) 2 (bits t);
   assert (v n.[0] % 2 = 1); // since bn_v n % 2 = 1
-  mod_inv_u64_lemma n.[0];
+  mod_inv_limb_lemma n.[0];
 
-  let aM0 = to_mont #nLen n mu r2 a in
-  to_mont_lemma #nLen n mu r2 a;
+  let aM0 = to_mont n mu r2 a in
+  to_mont_lemma n mu r2 a;
 
-  let accM0 = to_mont #nLen n mu r2 acc in
-  to_mont_lemma #nLen n mu r2 acc;
+  let accM0 = to_mont n mu r2 acc in
+  to_mont_lemma n mu r2 acc;
 
-  let (aM1, accM1) = repeati bBits (bn_mod_exp_f #nLen n mu bBits bLen b) (aM0, accM0) in
-  bn_mod_exp_mont_loop_lemma #nLen n mu bBits bLen b bBits (aM0, accM0);
+  let (aM1, accM1) = repeati bBits (bn_mod_exp_f n mu bBits bLen b) (aM0, accM0) in
+  bn_mod_exp_mont_loop_lemma n mu bBits bLen b bBits (aM0, accM0);
 
   let res = from_mont n mu accM1 in
-  from_mont_lemma #nLen n mu accM1
+  from_mont_lemma n mu accM1
 
 
-let bn_mod_exp_precompr2_lemma nLen n a bBits b r2 =
-  let mu = mod_inv_u64 n.[0] in
+let bn_mod_exp_precompr2_lemma #t nLen n a bBits b r2 =
+  let mu = mod_inv_limb n.[0] in
   let res1 = bn_mod_exp_precompr2 nLen n a bBits b r2 in
-  let res2 = BL.mod_exp_mont_ll nLen (bn_v n) (v mu) (bn_v a) bBits (bn_v b) in
+  let res2 = BL.mod_exp_mont_ll (bits t) nLen (bn_v n) (v mu) (bn_v a) bBits (bn_v b) in
   bn_mod_exp_mont_lemma_aux nLen n a bBits b r2;
   assert (bn_v res1 == res2 /\ bn_v res1 < bn_v n);
 
   bn_eval_index n 0;
-  assert (bn_v n % pow2 64 == v n.[0]);
-  Math.Lemmas.pow2_modulo_modulo_lemma_1 (bn_v n) 2 64;
+  assert (bn_v n % pow2 (bits t) == v n.[0]);
+  Math.Lemmas.pow2_modulo_modulo_lemma_1 (bn_v n) 2 (bits t);
   assert (v n.[0] % 2 = 1); // since bn_v n % 2 = 1
-  mod_inv_u64_lemma n.[0];
-  assert ((1 + (bn_v n % pow2 64) * v mu) % pow2 64 == 0);
+  mod_inv_limb_lemma n.[0];
+  assert ((1 + (bn_v n % pow2 (bits t)) * v mu) % pow2 (bits t) == 0);
 
   bn_eval_bound n nLen;
-  let d, k = M.eea_pow2_odd (64 * nLen) (bn_v n) in
-  M.mont_preconditions nLen (bn_v n) (v mu);
-  BL.mod_exp_mont_ll_lemma nLen (bn_v n) d (v mu) (bn_v a) bBits (bn_v b)
+  let d, k = M.eea_pow2_odd (bits t * nLen) (bn_v n) in
+  M.mont_preconditions (bits t) nLen (bn_v n) (v mu);
+  BL.mod_exp_mont_ll_lemma (bits t) nLen (bn_v n) d (v mu) (bn_v a) bBits (bn_v b)
 
 ///
 ///  Montgomery ladder for exponentiation
 ///
 
-let bn_mod_exp_mont_ladder_t (nLen:size_pos) (bBits:size_pos) (i:nat{i <= bBits}) =
-  tuple3 (lbignum nLen) (lbignum nLen) uint64
+let bn_mod_exp_mont_ladder_t (t:limb_t) (nLen:size_pos) (bBits:size_pos) (i:nat{i <= bBits}) =
+  tuple3 (lbignum t nLen) (lbignum t nLen) (limb t)
 
 val bn_mod_exp_mont_ladder_f:
-    #nLen:size_pos{nLen + nLen <= max_size_t}
-  -> n:lbignum nLen
-  -> mu:uint64
+    #t:limb_t
+  -> #nLen:size_pos{nLen + nLen <= max_size_t}
+  -> n:lbignum t nLen
+  -> mu:limb t
   -> bBits:size_pos
-  -> bLen:size_nat{bLen == blocks bBits 64}
-  -> b:lbignum bLen
+  -> bLen:size_nat{bLen == blocks bBits (bits t)}
+  -> b:lbignum t bLen
   -> i:nat{i < bBits}
-  -> rM0_rM1_privbit: tuple3 (lbignum nLen) (lbignum nLen) uint64 ->
-  tuple3 (lbignum nLen) (lbignum nLen) uint64
+  -> rM0_rM1_privbit: tuple3 (lbignum t nLen) (lbignum t nLen) (limb t) ->
+  tuple3 (lbignum t nLen) (lbignum t nLen) (limb t)
 
-let bn_mod_exp_mont_ladder_f #nLen n mu bBits bLen b i (rM0, rM1, privbit) =
-  let bit = bn_get_ith_bit #bLen b (bBits - i - 1) in
+let bn_mod_exp_mont_ladder_f #t #nLen n mu bBits bLen b i (rM0, rM1, privbit) =
+  let bit = bn_get_ith_bit b (bBits - i - 1) in
   let sw = bit ^. privbit in
   let rM0, rM1 = cswap2 sw rM0 rM1 in
   let rM0' = mont_sqr n mu rM0 in // rM0 * rM0 % n
@@ -260,217 +280,231 @@ let bn_mod_exp_mont_ladder_f #nLen n mu bBits bLen b i (rM0, rM1, privbit) =
 
 
 val bn_mod_exp_mont_ladder_:
-    nLen:size_pos{128 * nLen <= max_size_t}
-  -> n:lbignum nLen
-  -> a:lbignum nLen
-  -> acc:lbignum nLen
+    #t:limb_t
+  -> nLen:size_pos{2 * bits t * nLen <= max_size_t}
+  -> n:lbignum t nLen
+  -> a:lbignum t nLen
+  -> acc:lbignum t nLen
   -> bBits:size_pos
-  -> b:lbignum (blocks bBits 64)
-  -> r2:lbignum nLen ->
-  lbignum nLen
+  -> b:lbignum t (blocks bBits (bits t))
+  -> r2:lbignum t nLen ->
+  lbignum t nLen
 
-let bn_mod_exp_mont_ladder_ nLen n a one bBits b r2 =
-  let bLen = blocks bBits 64 in
-  let mu = mod_inv_u64 n.[0] in
+let bn_mod_exp_mont_ladder_ #t nLen n a one bBits b r2 =
+  let bLen = blocks bBits (bits t) in
+  let mu = mod_inv_limb n.[0] in
 
   let rM0 = to_mont n mu r2 one in
   let rM1 = to_mont n mu r2 a in
-  let sw = u64 0 in
-  let (rM0', rM1', sw') = repeat_gen bBits (bn_mod_exp_mont_ladder_t nLen bBits)
-    (bn_mod_exp_mont_ladder_f #nLen n mu bBits bLen b) (rM0, rM1, sw) in
+  let sw = uint #t 0 in
+  let (rM0', rM1', sw') = repeat_gen bBits (bn_mod_exp_mont_ladder_t t nLen bBits)
+    (bn_mod_exp_mont_ladder_f n mu bBits bLen b) (rM0, rM1, sw) in
   let (rM0', rM1') = cswap2 sw' rM0' rM1' in
   from_mont n mu rM0'
 
 
-let bn_mod_exp_mont_ladder_precompr2 nLen n a bBits b r2 =
-  let acc = bn_from_uint nLen (u64 1) in
+let bn_mod_exp_mont_ladder_precompr2 #t nLen n a bBits b r2 =
+  let acc = bn_from_uint nLen (uint #t 1) in
   bn_mod_exp_mont_ladder_ nLen n a acc bBits b r2
 
 
-val lemma_bit_xor_is_sum_mod2: a:uint64 -> b:uint64 -> Lemma
+val lemma_bit_xor_is_sum_mod2: #t:limb_t -> a:limb t -> b:limb t -> Lemma
   (requires v a <= 1 /\ v b <= 1)
   (ensures  v (a ^. b) == (v a + v b) % 2)
 
-let lemma_bit_xor_is_sum_mod2 a b =
-  logxor_spec a b;
-  assert_norm (UInt64.logxor 0uL 0uL == 0uL);
-  assert_norm (UInt64.logxor 0uL 1uL == 1uL);
-  assert_norm (UInt64.logxor 1uL 0uL == 1uL);
-  assert_norm (UInt64.logxor 1uL 1uL == 0uL)
+let lemma_bit_xor_is_sum_mod2 #t a b =
+  match t with
+  | U32 ->
+    logxor_spec a b;
+    assert_norm (UInt32.logxor 0ul 0ul == 0ul);
+    assert_norm (UInt32.logxor 0ul 1ul == 1ul);
+    assert_norm (UInt32.logxor 1ul 0ul == 1ul);
+    assert_norm (UInt32.logxor 1ul 1ul == 0ul)
+  | U64 ->
+    logxor_spec a b;
+    assert_norm (UInt64.logxor 0uL 0uL == 0uL);
+    assert_norm (UInt64.logxor 0uL 1uL == 1uL);
+    assert_norm (UInt64.logxor 1uL 0uL == 1uL);
+    assert_norm (UInt64.logxor 1uL 1uL == 0uL)
 
 
 val bn_mod_exp_mont_ladder_f_lemma:
-    #nLen:size_pos{nLen + nLen <= max_size_t}
-  -> n:lbignum nLen
-  -> mu:uint64
+    #t:limb_t
+  -> #nLen:size_pos{nLen + nLen <= max_size_t}
+  -> n:lbignum t nLen
+  -> mu:limb t
   -> bBits:size_pos
-  -> bLen:size_nat{bLen == blocks bBits 64}
-  -> b:lbignum bLen
+  -> bLen:size_nat{bLen == blocks bBits (bits t)}
+  -> b:lbignum t bLen
   -> i:nat{i < bBits}
-  -> rM0_rM1_sw: tuple3 (lbignum nLen) (lbignum nLen) uint64 -> Lemma
+  -> rM0_rM1_sw: tuple3 (lbignum t nLen) (lbignum t nLen) (limb t) -> Lemma
   (requires
    (let (rM0, rM1, sw) = rM0_rM1_sw in
-    (1 + (bn_v n % pow2 64) * v mu) % pow2 64 == 0 /\
+    (1 + (bn_v n % pow2 (bits t)) * v mu) % pow2 (bits t) == 0 /\
     bn_v n % 2 = 1 /\ 1 < bn_v n /\
     0 < bn_v b /\ bn_v b < pow2 bBits /\
     bn_v rM0 < bn_v n /\ bn_v rM1 < bn_v n /\ v sw <= 1))
   (ensures
    (let (rM0, rM1, sw) = rM0_rM1_sw in
-    let (rM0', rM1', sw') = bn_mod_exp_mont_ladder_f #nLen n mu bBits bLen b i (rM0, rM1, sw) in
-    let (rM0'', rM1'', sw'') = BL.mod_exp_mont_ladder_swap_f_ll nLen (bn_v n) (v mu) bBits (bn_v b) i (bn_v rM0, bn_v rM1, v sw) in
+    let (rM0', rM1', sw') = bn_mod_exp_mont_ladder_f n mu bBits bLen b i (rM0, rM1, sw) in
+    let (rM0'', rM1'', sw'') = BL.mod_exp_mont_ladder_swap_f_ll (bits t) nLen (bn_v n) (v mu) bBits (bn_v b) i (bn_v rM0, bn_v rM1, v sw) in
     bn_v rM0' == rM0'' /\ bn_v rM1' == rM1'' /\ v sw' == sw'' /\
     bn_v rM0' < bn_v n /\ bn_v rM1' < bn_v n /\ v sw' <= 1))
 
-let bn_mod_exp_mont_ladder_f_lemma #nLen n mu bBits bLen b i (rM0, rM1, sw) =
-  let (rM0', rM1', sw') = bn_mod_exp_mont_ladder_f #nLen n mu bBits bLen b i (rM0, rM1, sw) in
-  let (rM0'', rM1'', sw'') = BL.mod_exp_mont_ladder_swap_f_ll nLen (bn_v n) (v mu) bBits (bn_v b) i (bn_v rM0, bn_v rM1, v sw) in
-  let bit = bn_get_ith_bit #bLen b (bBits - i - 1) in
-  bn_get_ith_bit_lemma #bLen b (bBits - i - 1);
+let bn_mod_exp_mont_ladder_f_lemma #t #nLen n mu bBits bLen b i (rM0, rM1, sw) =
+  let (rM0', rM1', sw') = bn_mod_exp_mont_ladder_f n mu bBits bLen b i (rM0, rM1, sw) in
+  let (rM0'', rM1'', sw'') = BL.mod_exp_mont_ladder_swap_f_ll (bits t) nLen (bn_v n) (v mu) bBits (bn_v b) i (bn_v rM0, bn_v rM1, v sw) in
+  let bit = bn_get_ith_bit b (bBits - i - 1) in
+  bn_get_ith_bit_lemma b (bBits - i - 1);
   //assert (v bit == bn_v b / pow2 (bBits - i - 1) % 2);
   let sw1 = bit ^. sw in
   lemma_bit_xor_is_sum_mod2 bit sw;
   let rM2, rM3 = cswap2 sw1 rM0 rM1 in
   cswap2_lemma sw1 rM0 rM1;
   let rM2' = mont_sqr n mu rM2 in
-  mont_sqr_lemma #nLen n mu rM2;
+  mont_sqr_lemma n mu rM2;
   let rM3' = mont_mul n mu rM3 rM2 in
-  mont_mul_lemma #nLen n mu rM3 rM2;
+  mont_mul_lemma n mu rM3 rM2;
   assert (rM0' == rM2' /\ rM1' == rM3' /\ sw' == bit);
   assert (bn_v rM0' == rM0'' /\ bn_v rM1' == rM1'' /\ v sw' == sw'')
 
 
 val bn_mod_exp_mont_ladder_loop_lemma:
-    #nLen:size_pos{nLen + nLen <= max_size_t}
-  -> n:lbignum nLen
-  -> mu:uint64
+    #t:limb_t
+  -> #nLen:size_pos{nLen + nLen <= max_size_t}
+  -> n:lbignum t nLen
+  -> mu:limb t
   -> bBits:size_pos
-  -> bLen:size_nat{bLen == blocks bBits 64}
-  -> b:lbignum bLen
+  -> bLen:size_nat{bLen == blocks bBits (bits t)}
+  -> b:lbignum t bLen
   -> i:size_nat{i <= bBits}
-  -> rM0_rM1_sw: tuple3 (lbignum nLen) (lbignum nLen) uint64 -> Lemma
+  -> rM0_rM1_sw: tuple3 (lbignum t nLen) (lbignum t nLen) (limb t) -> Lemma
   (requires
    (let (rM0, rM1, sw) = rM0_rM1_sw in
-    (1 + (bn_v n % pow2 64) * v mu) % pow2 64 == 0 /\
+    (1 + (bn_v n % pow2 (bits t)) * v mu) % pow2 (bits t) == 0 /\
     bn_v n % 2 = 1 /\ 1 < bn_v n /\
     0 < bn_v b /\ bn_v b < pow2 bBits /\
     bn_v rM0 < bn_v n /\ bn_v rM1 < bn_v n /\ v sw <= 1))
   (ensures
    (let (rM0, rM1, sw) = rM0_rM1_sw in
-    let (rM0', rM1', sw') = repeat_gen i (bn_mod_exp_mont_ladder_t nLen bBits)
-      (bn_mod_exp_mont_ladder_f #nLen n mu bBits bLen b) (rM0, rM1, sw) in
-    let (rM0'', rM1'', sw'') = repeati i (BL.mod_exp_mont_ladder_swap_f_ll nLen (bn_v n) (v mu) bBits (bn_v b)) (bn_v rM0, bn_v rM1, v sw) in
+    let (rM0', rM1', sw') = repeat_gen i (bn_mod_exp_mont_ladder_t t nLen bBits)
+      (bn_mod_exp_mont_ladder_f n mu bBits bLen b) (rM0, rM1, sw) in
+    let (rM0'', rM1'', sw'') = repeati i
+      (BL.mod_exp_mont_ladder_swap_f_ll (bits t) nLen (bn_v n) (v mu) bBits (bn_v b)) (bn_v rM0, bn_v rM1, v sw) in
     bn_v rM0' == rM0'' /\ bn_v rM1' == rM1'' /\ v sw' == sw'' /\
     bn_v rM0' < bn_v n /\ bn_v rM1' < bn_v n /\ v sw' <= 1))
 
-let rec bn_mod_exp_mont_ladder_loop_lemma #nLen n mu bBits bLen b i (rM0, rM1, sw) =
-  let (rM0', rM1', sw') = repeat_gen i (bn_mod_exp_mont_ladder_t nLen bBits)
-      (bn_mod_exp_mont_ladder_f #nLen n mu bBits bLen b) (rM0, rM1, sw) in
-  let (rM0'', rM1'', sw'') = repeati i (BL.mod_exp_mont_ladder_swap_f_ll nLen (bn_v n) (v mu) bBits (bn_v b)) (bn_v rM0, bn_v rM1, v sw) in
+let rec bn_mod_exp_mont_ladder_loop_lemma #t #nLen n mu bBits bLen b i (rM0, rM1, sw) =
+  let (rM0', rM1', sw') = repeat_gen i (bn_mod_exp_mont_ladder_t t nLen bBits)
+      (bn_mod_exp_mont_ladder_f n mu bBits bLen b) (rM0, rM1, sw) in
+  let (rM0'', rM1'', sw'') = repeati i
+    (BL.mod_exp_mont_ladder_swap_f_ll (bits t) nLen (bn_v n) (v mu) bBits (bn_v b)) (bn_v rM0, bn_v rM1, v sw) in
 
   if i = 0 then begin
-    eq_repeat_gen0 i (bn_mod_exp_mont_ladder_t nLen bBits) (bn_mod_exp_mont_ladder_f #nLen n mu bBits bLen b) (rM0, rM1, sw);
-    eq_repeati0 i (BL.mod_exp_mont_ladder_swap_f_ll nLen (bn_v n) (v mu) bBits (bn_v b)) (bn_v rM0, bn_v rM1, v sw);
+    eq_repeat_gen0 i (bn_mod_exp_mont_ladder_t t nLen bBits) (bn_mod_exp_mont_ladder_f n mu bBits bLen b) (rM0, rM1, sw);
+    eq_repeati0 i (BL.mod_exp_mont_ladder_swap_f_ll (bits t) nLen (bn_v n) (v mu) bBits (bn_v b)) (bn_v rM0, bn_v rM1, v sw);
     () end
   else begin
-    unfold_repeat_gen i (bn_mod_exp_mont_ladder_t nLen bBits) (bn_mod_exp_mont_ladder_f #nLen n mu bBits bLen b) (rM0, rM1, sw) (i - 1);
-    unfold_repeati i (BL.mod_exp_mont_ladder_swap_f_ll nLen (bn_v n) (v mu) bBits (bn_v b)) (bn_v rM0, bn_v rM1, v sw) (i - 1);
+    unfold_repeat_gen i (bn_mod_exp_mont_ladder_t t nLen bBits) (bn_mod_exp_mont_ladder_f n mu bBits bLen b) (rM0, rM1, sw) (i - 1);
+    unfold_repeati i (BL.mod_exp_mont_ladder_swap_f_ll (bits t) nLen (bn_v n) (v mu) bBits (bn_v b)) (bn_v rM0, bn_v rM1, v sw) (i - 1);
 
-    let (rM2', rM3', sw1') = repeat_gen (i - 1) (bn_mod_exp_mont_ladder_t nLen bBits)
-      (bn_mod_exp_mont_ladder_f #nLen n mu bBits bLen b) (rM0, rM1, sw) in
-    let (rM2'', rM3'', sw1'') = repeati (i - 1) (BL.mod_exp_mont_ladder_swap_f_ll nLen (bn_v n) (v mu) bBits (bn_v b)) (bn_v rM0, bn_v rM1, v sw) in
-    assert ((rM0', rM1', sw') == bn_mod_exp_mont_ladder_f #nLen n mu bBits bLen b (i - 1) (rM2', rM3', sw1'));
-    assert ((rM0'', rM1'', sw'') == BL.mod_exp_mont_ladder_swap_f_ll nLen (bn_v n) (v mu) bBits (bn_v b) (i - 1) (rM2'', rM3'', sw1''));
-    bn_mod_exp_mont_ladder_loop_lemma #nLen n mu bBits bLen b (i - 1) (rM0, rM1, sw);
+    let (rM2', rM3', sw1') = repeat_gen (i - 1) (bn_mod_exp_mont_ladder_t t nLen bBits)
+      (bn_mod_exp_mont_ladder_f n mu bBits bLen b) (rM0, rM1, sw) in
+    let (rM2'', rM3'', sw1'') = repeati (i - 1) (BL.mod_exp_mont_ladder_swap_f_ll (bits t) nLen (bn_v n) (v mu) bBits (bn_v b)) (bn_v rM0, bn_v rM1, v sw) in
+    assert ((rM0', rM1', sw') == bn_mod_exp_mont_ladder_f n mu bBits bLen b (i - 1) (rM2', rM3', sw1'));
+    assert ((rM0'', rM1'', sw'') == BL.mod_exp_mont_ladder_swap_f_ll (bits t) nLen (bn_v n) (v mu) bBits (bn_v b) (i - 1) (rM2'', rM3'', sw1''));
+    bn_mod_exp_mont_ladder_loop_lemma n mu bBits bLen b (i - 1) (rM0, rM1, sw);
     assert (bn_v rM2' == rM2'' /\ bn_v rM3' == rM3'' /\ v sw1' == sw1'');
-    bn_mod_exp_mont_ladder_f_lemma #nLen n mu bBits bLen b (i - 1) (rM2', rM3', sw1');
+    bn_mod_exp_mont_ladder_f_lemma n mu bBits bLen b (i - 1) (rM2', rM3', sw1');
     () end
 
 
 val bn_mod_exp_mont_ladder_lemma_aux:
-    nLen:size_pos{128 * nLen <= max_size_t}
-  -> n:lbignum nLen
-  -> a:lbignum nLen
+    #t:limb_t
+  -> nLen:size_pos{2 * bits t * nLen <= max_size_t}
+  -> n:lbignum t nLen
+  -> a:lbignum t nLen
   -> bBits:size_pos
-  -> b:lbignum (blocks bBits 64)
-  -> r2:lbignum nLen -> Lemma
+  -> b:lbignum t (blocks bBits (bits t))
+  -> r2:lbignum t nLen -> Lemma
   (requires
     bn_v n % 2 = 1 /\ 1 < bn_v n /\
     0 < bn_v b /\ bn_v b < pow2 bBits /\ bn_v a < bn_v n /\
-    bn_v r2 == pow2 (128 * nLen) % bn_v n)
+    bn_v r2 == pow2 (2 * bits t * nLen) % bn_v n)
   (ensures
-   (let mu = mod_inv_u64 n.[0] in
+   (let mu = mod_inv_limb n.[0] in
     let res1 = bn_mod_exp_mont_ladder_precompr2 nLen n a bBits b r2 in
-    let res2 = BL.mod_exp_mont_ladder_swap_ll nLen (bn_v n) (v mu) (bn_v a) bBits (bn_v b) in
+    let res2 = BL.mod_exp_mont_ladder_swap_ll (bits t) nLen (bn_v n) (v mu) (bn_v a) bBits (bn_v b) in
     bn_v res1 == res2 /\ bn_v res1 < bn_v n))
 
-let bn_mod_exp_mont_ladder_lemma_aux nLen n a bBits b r2 =
-  let bLen = blocks bBits 64 in
+let bn_mod_exp_mont_ladder_lemma_aux #t nLen n a bBits b r2 =
+  let bLen = blocks bBits (bits t) in
 
-  let one = bn_from_uint nLen (u64 1) in
-  bn_from_uint_lemma nLen (u64 1);
+  let one = bn_from_uint nLen (uint #t 1) in
+  bn_from_uint_lemma nLen (uint #t 1);
   assert (bn_v one == 1);
 
-  let mu = mod_inv_u64 n.[0] in
+  let mu = mod_inv_limb n.[0] in
   bn_eval_index n 0;
-  assert (bn_v n % pow2 64 == v n.[0]);
-  Math.Lemmas.pow2_modulo_modulo_lemma_1 (bn_v n) 2 64;
+  assert (bn_v n % pow2 (bits t) == v n.[0]);
+  Math.Lemmas.pow2_modulo_modulo_lemma_1 (bn_v n) 2 (bits t);
   assert (v n.[0] % 2 = 1); // since bn_v n % 2 = 1
-  mod_inv_u64_lemma n.[0];
+  mod_inv_limb_lemma n.[0];
 
-  let rM0 = to_mont #nLen n mu r2 one in
-  to_mont_lemma #nLen n mu r2 one;
+  let rM0 = to_mont n mu r2 one in
+  to_mont_lemma n mu r2 one;
 
-  let rM1 = to_mont #nLen n mu r2 a in
-  to_mont_lemma #nLen n mu r2 a;
+  let rM1 = to_mont n mu r2 a in
+  to_mont_lemma n mu r2 a;
 
-  let sw = u64 0 in
-  let (rM0', rM1', sw') = repeat_gen bBits (bn_mod_exp_mont_ladder_t nLen bBits)
-    (bn_mod_exp_mont_ladder_f #nLen n mu bBits bLen b) (rM0, rM1, sw) in
-  bn_mod_exp_mont_ladder_loop_lemma #nLen n mu bBits bLen b bBits (rM0, rM1, sw);
+  let sw = uint #t 0 in
+  let (rM0', rM1', sw') = repeat_gen bBits (bn_mod_exp_mont_ladder_t t nLen bBits)
+    (bn_mod_exp_mont_ladder_f n mu bBits bLen b) (rM0, rM1, sw) in
+  bn_mod_exp_mont_ladder_loop_lemma n mu bBits bLen b bBits (rM0, rM1, sw);
 
   let (rM0'', rM1'') = cswap2 sw' rM0' rM1' in
   cswap2_lemma sw' rM0' rM1';
   let res = from_mont n mu rM0'' in
-  from_mont_lemma #nLen n mu rM0''
+  from_mont_lemma n mu rM0''
 
 
-let bn_mod_exp_mont_ladder_precompr2_lemma nLen n a bBits b r2 =
-  let mu = mod_inv_u64 n.[0] in
+let bn_mod_exp_mont_ladder_precompr2_lemma #t nLen n a bBits b r2 =
+  let mu = mod_inv_limb n.[0] in
   let res1 = bn_mod_exp_mont_ladder_precompr2 nLen n a bBits b r2 in
-  let res2 = BL.mod_exp_mont_ladder_swap_ll nLen (bn_v n) (v mu) (bn_v a) bBits (bn_v b) in
+  let res2 = BL.mod_exp_mont_ladder_swap_ll (bits t) nLen (bn_v n) (v mu) (bn_v a) bBits (bn_v b) in
   bn_mod_exp_mont_ladder_lemma_aux nLen n a bBits b r2;
   assert (bn_v res1 == res2 /\ bn_v res1 < bn_v n);
 
   bn_eval_index n 0;
-  assert (bn_v n % pow2 64 == v n.[0]);
-  Math.Lemmas.pow2_modulo_modulo_lemma_1 (bn_v n) 2 64;
+  assert (bn_v n % pow2 (bits t) == v n.[0]);
+  Math.Lemmas.pow2_modulo_modulo_lemma_1 (bn_v n) 2 (bits t);
   assert (v n.[0] % 2 = 1); // since bn_v n % 2 = 1
-  mod_inv_u64_lemma n.[0];
-  assert ((1 + (bn_v n % pow2 64) * v mu) % pow2 64 == 0);
+  mod_inv_limb_lemma n.[0];
+  assert ((1 + (bn_v n % pow2 (bits t)) * v mu) % pow2 (bits t) == 0);
 
   bn_eval_bound n nLen;
-  let d, k = M.eea_pow2_odd (64 * nLen) (bn_v n) in
-  M.mont_preconditions nLen (bn_v n) (v mu);
-  BL.mod_exp_mont_ladder_swap_ll_lemma nLen (bn_v n) d (v mu) (bn_v a) bBits (bn_v b)
+  let d, k = M.eea_pow2_odd (bits t * nLen) (bn_v n) in
+  M.mont_preconditions (bits t) nLen (bn_v n) (v mu);
+  BL.mod_exp_mont_ladder_swap_ll_lemma (bits t) nLen (bn_v n) d (v mu) (bn_v a) bBits (bn_v b)
 
 
-let bn_mod_exp nLen n a bBits b =
+let bn_mod_exp #t nLen n a bBits b =
   let r2 = precomp_r2_mod_n n in
   bn_mod_exp_precompr2 nLen n a bBits b r2
 
 
-let bn_mod_exp_lemma nLen n a bBits b =
+let bn_mod_exp_lemma #t nLen n a bBits b =
   let r2 = precomp_r2_mod_n n in
   precomp_r2_mod_n_lemma n;
   bn_mod_exp_precompr2_lemma nLen n a bBits b r2
 
 
-let bn_mod_exp_mont_ladder nLen n a bBits b =
+let bn_mod_exp_mont_ladder #t nLen n a bBits b =
   let r2 = precomp_r2_mod_n n in
   bn_mod_exp_mont_ladder_precompr2 nLen n a bBits b r2
 
 
-let bn_mod_exp_mont_ladder_lemma nLen n a bBits b =
+let bn_mod_exp_mont_ladder_lemma #t nLen n a bBits b =
   let r2 = precomp_r2_mod_n n in
   precomp_r2_mod_n_lemma n;
   bn_mod_exp_mont_ladder_precompr2_lemma nLen n a bBits b r2
