code/bignum/Hacl.Spec.Bignum.ModInv.fst
@@ -47,41 +47,43 @@ let mod_inv_prime_lemma n a =
 
 
 val bn_mod_inv_prime:
-    #nLen:size_pos{128 * nLen <= max_size_t}
-  -> n:lbignum nLen
-  -> a:lbignum nLen ->
-  lbignum nLen
+    #t:limb_t
+  -> #nLen:size_pos{2 * bits t * nLen <= max_size_t}
+  -> n:lbignum t nLen
+  -> a:lbignum t nLen ->
+  lbignum t nLen
 
-let bn_mod_inv_prime #nLen n a =
-  let b2 = create 1 (u64 2) in
+let bn_mod_inv_prime #t #nLen n a =
+  let b2 = create 1 (uint #t 2) in
   let c, n2 = bn_sub n b2 in
-  BE.bn_mod_exp nLen n a (64 * nLen) n2
+  BE.bn_mod_exp nLen n a (bits t * nLen) n2
 
 
 val bn_mod_inv_prime_lemma:
-    #nLen:size_pos{128 * nLen <= max_size_t}
-  -> n:lbignum nLen
-  -> a:lbignum nLen -> Lemma
+    #t:limb_t
+  -> #nLen:size_pos{2 * bits t * nLen <= max_size_t}
+  -> n:lbignum t nLen
+  -> a:lbignum t nLen -> Lemma
   (requires
     bn_v n % 2 = 1 /\ 1 < bn_v n /\
     0 < bn_v a /\ bn_v a < bn_v n /\
     Euclid.is_prime (bn_v n))
   (ensures  (bn_v (bn_mod_inv_prime n a) * bn_v a % bn_v n = 1))
 
-let bn_mod_inv_prime_lemma #nLen n a =
-  let b2 = create 1 (u64 2) in
+let bn_mod_inv_prime_lemma #t #nLen n a =
+  let b2 = create 1 (uint #t 2) in
   bn_eval1 b2;
   assert (bn_v b2 = 2);
 
   let c, n2 = bn_sub n b2 in
   bn_sub_lemma n b2;
-  assert (bn_v n2 - v c * pow2 (64 * nLen) == bn_v n - 2);
+  assert (bn_v n2 - v c * pow2 (bits t * nLen) == bn_v n - 2);
   bn_eval_bound n2 nLen;
   bn_eval_bound n nLen;
   assert (v c = 0);
   assert (bn_v n2 == bn_v n - 2);
 
-  let res = BE.bn_mod_exp nLen n a (64 * nLen) n2 in
-  BE.bn_mod_exp_lemma nLen n a (64 * nLen) n2;
+  let res = BE.bn_mod_exp nLen n a (bits t * nLen) n2 in
+  BE.bn_mod_exp_lemma nLen n a (bits t * nLen) n2;
   assert (bn_v res == Lib.NatMod.pow_mod #(bn_v n) (bn_v a) (bn_v n2));
   mod_inv_prime_lemma (bn_v n) (bn_v a)
