code/bignum/Hacl.Spec.Bignum.ModReduction.fst
@@ -9,7 +9,7 @@ open Hacl.Spec.Bignum.Definitions
 
 module M = Hacl.Spec.Montgomery.Lemmas
 module BM = Hacl.Spec.Bignum.Montgomery
-module BI = Hacl.Spec.Bignum.ModInv64
+module BI = Hacl.Spec.Bignum.ModInvLimb
 module BN = Hacl.Spec.Bignum
 
 #reset-options "--z3rlimit 50 --fuel 0 --ifuel 0"
@@ -19,14 +19,15 @@ module BN = Hacl.Spec.Bignum
 ///
 
 val check_bn_mod:
-    #nLen:size_pos{128 * nLen <= max_size_t}
-  -> n:lbignum nLen
-  -> a:lbignum (nLen + nLen) ->
-  res:uint64{
+    #t:limb_t
+  -> #nLen:size_pos{2 * bits t * nLen <= max_size_t}
+  -> n:lbignum t nLen
+  -> a:lbignum t (nLen + nLen) ->
+  res:limb t{
     let b = 1 < bn_v n && bn_v n % 2 = 1 && bn_v a < bn_v n * bn_v n in
-    v res == (if b then v (ones U64 SEC) else v (zeros U64 SEC))}
+    v res == (if b then v (ones t SEC) else v (zeros t SEC))}
 
-let check_bn_mod #nLen n a =
+let check_bn_mod #t #nLen n a =
   let m0 = BM.check_modulus n in
   let n2 = BN.bn_mul n n in
   BN.bn_mul_lemma n n;
@@ -38,36 +39,38 @@ let check_bn_mod #nLen n a =
 
 // TODO: we can pass a constant mu as well
 val bn_mod_slow_precompr2:
-    #nLen:size_pos{128 * nLen <= max_size_t}
-  -> n:lbignum nLen
-  -> a:lbignum (nLen + nLen)
-  -> r2:lbignum nLen ->
-  lbignum nLen
+    #t:limb_t
+  -> #nLen:size_pos{2 * bits t * nLen <= max_size_t}
+  -> n:lbignum t nLen
+  -> a:lbignum t (nLen + nLen)
+  -> r2:lbignum t nLen ->
+  lbignum t nLen
 
-let bn_mod_slow_precompr2 #nLen n a r2 =
-  let mu = BI.mod_inv_u64 n.[0] in
+let bn_mod_slow_precompr2 #t #nLen n a r2 =
+  let mu = BI.mod_inv_limb n.[0] in
   let a_mod = BM.mont_reduction n mu a in
   let res = BM.to_mont n mu r2 a_mod in
   res
 
 
 val bn_mod_slow_precompr2_lemma:
-    #nLen:size_pos{128 * nLen <= max_size_t}
-  -> n:lbignum nLen
-  -> a:lbignum (nLen + nLen)
-  -> r2:lbignum nLen -> Lemma
+    #t:limb_t
+  -> #nLen:size_pos{2 * bits t * nLen <= max_size_t}
+  -> n:lbignum t nLen
+  -> a:lbignum t (nLen + nLen)
+  -> r2:lbignum t nLen -> Lemma
   (requires
     1 < bn_v n /\ bn_v n % 2 = 1 /\ bn_v a < bn_v n * bn_v n /\
-    bn_v r2 == pow2 (128 * nLen) % bn_v n)
+    bn_v r2 == pow2 (2 * bits t * nLen) % bn_v n)
   (ensures bn_v (bn_mod_slow_precompr2 n a r2) == bn_v a % bn_v n)
 
-let bn_mod_slow_precompr2_lemma #nLen n a r2 =
-  let mu = BI.mod_inv_u64 n.[0] in
+let bn_mod_slow_precompr2_lemma #t #nLen n a r2 =
+  let mu = BI.mod_inv_limb n.[0] in
   bn_eval_index n 0;
-  assert (bn_v n % pow2 64 == v n.[0]);
-  Math.Lemmas.pow2_modulo_modulo_lemma_1 (bn_v n) 2 64;
+  assert (bn_v n % pow2 (bits t) == v n.[0]);
+  Math.Lemmas.pow2_modulo_modulo_lemma_1 (bn_v n) 2 (bits t);
   assert (v n.[0] % 2 = 1); // since bn_v n % 2 = 1
-  BI.mod_inv_u64_lemma n.[0];
+  BI.mod_inv_limb_lemma n.[0];
 
   let a_mod = BM.mont_reduction n mu a in
   let res = BM.to_mont n mu r2 a_mod in
@@ -75,12 +78,12 @@ let bn_mod_slow_precompr2_lemma #nLen n a r2 =
   BM.mont_reduction_lemma n mu a;
   BM.to_mont_lemma n mu r2 a_mod;
 
-  let d, k = M.eea_pow2_odd (64 * nLen) (bn_v n) in
-  M.mont_preconditions nLen (bn_v n) (v mu);
-  M.mont_reduction_lemma nLen (bn_v n) d (v mu) (bn_v a);
+  let d, k = M.eea_pow2_odd (bits t * nLen) (bn_v n) in
+  M.mont_preconditions (bits t) nLen (bn_v n) (v mu);
+  M.mont_reduction_lemma (bits t) nLen (bn_v n) d (v mu) (bn_v a);
   assert (bn_v a_mod == bn_v a * d % bn_v n);
-  M.to_mont_lemma nLen (bn_v n) d (v mu) (bn_v a_mod);
-  let r = pow2 (64 * nLen) in
+  M.to_mont_lemma (bits t) nLen (bn_v n) d (v mu) (bn_v a_mod);
+  let r = pow2 (bits t * nLen) in
   assert (bn_v res == bn_v a_mod * r % bn_v n);
   M.lemma_mont_id1 (bn_v n) r d (bn_v a);
   assert (bn_v res == bn_v a % bn_v n)
