code/bignum/Hacl.Spec.Montgomery.Lemmas.fst
@@ -123,14 +123,14 @@ let eea_pow2_odd a n =
   (- d, - k)
 
 
-val mont_preconditions_d: rLen:pos -> n:pos{n > 1} -> Lemma
+val mont_preconditions_d: pbits:pos -> rLen:pos -> n:pos{n > 1} -> Lemma
   (requires  n % 2 = 1)
-  (ensures  (let d, k = eea_pow2_odd (64 * rLen) n in pow2 (64 * rLen) * d % n == 1))
+  (ensures  (let d, k = eea_pow2_odd (pbits * rLen) n in pow2 (pbits * rLen) * d % n == 1))
 
-let mont_preconditions_d rLen n =
-  let d, k = eea_pow2_odd (64 * rLen) n in
+let mont_preconditions_d pbits rLen n =
+  let d, k = eea_pow2_odd (pbits * rLen) n in
   calc (==) {
-    pow2 (64 * rLen) * d % n;
+    pow2 (pbits * rLen) * d % n;
     (==) { }
     (1 + k * n) % n;
     (==) { Math.Lemmas.modulo_addition_lemma 1 n k }
@@ -138,69 +138,70 @@ let mont_preconditions_d rLen n =
     (==) { Math.Lemmas.small_mod 1 n }
     1;
   };
-  assert (pow2 (64 * rLen) * d % n == 1)
+  assert (pow2 (pbits * rLen) * d % n == 1)
 
 
-val mont_preconditions_n0: n:pos{n > 1} -> mu:nat -> Lemma
-  (requires (1 + (n % pow2 64) * mu) % pow2 64 == 0)
-  (ensures  (1 + n * mu) % pow2 64 == 0)
+val mont_preconditions_n0: pbits:pos -> n:pos{n > 1} -> mu:nat -> Lemma
+  (requires (1 + (n % pow2 pbits) * mu) % pow2 pbits == 0)
+  (ensures  (1 + n * mu) % pow2 pbits == 0)
 
-let mont_preconditions_n0 n mu =
+let mont_preconditions_n0 pbits n mu =
   calc (==) {
-    (1 + n * mu) % pow2 64;
-    (==) { Math.Lemmas.lemma_mod_plus_distr_r 1 (n * mu) (pow2 64) }
-    (1 + n * mu % pow2 64) % pow2 64;
-    (==) { Math.Lemmas.lemma_mod_mul_distr_l n mu (pow2 64) }
-    (1 + n % pow2 64 * mu % pow2 64) % pow2 64;
-    (==) { Math.Lemmas.lemma_mod_plus_distr_r 1 (n % pow2 64 * mu) (pow2 64) }
-    (1 + n % pow2 64 * mu) % pow2 64;
-    (==) { assert ((1 + (n % pow2 64) * mu) % pow2 64 == 0) }
+    (1 + n * mu) % pow2 pbits;
+    (==) { Math.Lemmas.lemma_mod_plus_distr_r 1 (n * mu) (pow2 pbits) }
+    (1 + n * mu % pow2 pbits) % pow2 pbits;
+    (==) { Math.Lemmas.lemma_mod_mul_distr_l n mu (pow2 pbits) }
+    (1 + n % pow2 pbits * mu % pow2 pbits) % pow2 pbits;
+    (==) { Math.Lemmas.lemma_mod_plus_distr_r 1 (n % pow2 pbits * mu) (pow2 pbits) }
+    (1 + n % pow2 pbits * mu) % pow2 pbits;
+    (==) { assert ((1 + (n % pow2 pbits) * mu) % pow2 pbits == 0) }
     0;
   };
-  assert ((1 + n * mu) % pow2 64 == 0)
+  assert ((1 + n * mu) % pow2 pbits == 0)
+
 
 val mont_preconditions:
-  nLen:nat -> n:pos{1 < n /\ n < pow2 (64 * nLen)} -> mu:nat -> Lemma
-  (requires n % 2 = 1 /\ (1 + (n % pow2 64) * mu) % pow2 64 == 0)
+  pbits:pos -> nLen:nat -> n:pos{1 < n /\ n < pow2 (pbits * nLen)} -> mu:nat -> Lemma
+  (requires n % 2 = 1 /\ (1 + (n % pow2 pbits) * mu) % pow2 pbits == 0)
   (ensures
-    (let r = pow2 (64 * nLen) in
-     let d, _ = eea_pow2_odd (64 * nLen) n in
-     r * d % n == 1 /\ n < r /\ (1 + n * mu) % pow2 64 == 0))
+    (let r = pow2 (pbits * nLen) in
+     let d, _ = eea_pow2_odd (pbits * nLen) n in
+     r * d % n == 1 /\ n < r /\ (1 + n * mu) % pow2 pbits == 0))
 
-let mont_preconditions nLen n mu =
-  mont_preconditions_d nLen n;
-  mont_preconditions_n0 n mu
+let mont_preconditions pbits nLen n mu =
+  mont_preconditions_d pbits nLen n;
+  mont_preconditions_n0 pbits n mu
 
 ///
 ///  High-level specification of Montgomery arithmetic
 ///
 
-val mont_reduction_f: rLen:nat -> n:pos -> mu:nat -> i:nat{i < rLen} -> c:nat -> nat
-let mont_reduction_f rLen n mu i c =
-  let c_i = c / pow2 (64 * i) % pow2 64 in
-  let q_i = mu * c_i % pow2 64 in
-  let res = c + n * q_i * pow2 (64 * i) in
+val mont_reduction_f: pbits:pos -> rLen:nat -> n:pos -> mu:nat -> i:nat{i < rLen} -> c:nat -> nat
+let mont_reduction_f pbits rLen n mu i c =
+  let c_i = c / pow2 (pbits * i) % pow2 pbits in
+  let q_i = mu * c_i % pow2 pbits in
+  let res = c + n * q_i * pow2 (pbits * i) in
   res
 
-val mont_reduction: rLen:nat -> n:pos -> mu:nat -> c:nat -> nat
-let mont_reduction rLen n mu c =
-  let res = repeati rLen (mont_reduction_f rLen n mu) c in
-  let res = res / pow2 (64 * rLen) in
+val mont_reduction: pbits:pos -> rLen:nat -> n:pos -> mu:nat -> c:nat -> nat
+let mont_reduction pbits rLen n mu c =
+  let res = repeati rLen (mont_reduction_f pbits rLen n mu) c in
+  let res = res / pow2 (pbits * rLen) in
   if res < n then res else res - n
 
-val to_mont: rLen:nat -> n:pos -> mu:nat -> a:nat -> nat
-let to_mont rLen n mu a =
-  let r2 = pow2 (128 * rLen) % n in
+val to_mont: pbits:pos -> rLen:nat -> n:pos -> mu:nat -> a:nat -> nat
+let to_mont pbits rLen n mu a =
+  let r2 = pow2 (2 * pbits * rLen) % n in
   let c = a * r2 in
-  mont_reduction rLen n mu c
+  mont_reduction pbits rLen n mu c
 
-val from_mont: rLen:nat -> n:pos -> mu:nat -> aM:nat -> nat
-let from_mont rLen n mu aM = mont_reduction rLen n mu aM
+val from_mont: pbits:pos -> rLen:nat -> n:pos -> mu:nat -> aM:nat -> nat
+let from_mont pbits rLen n mu aM = mont_reduction pbits rLen n mu aM
 
-val mont_mul: rLen:nat -> n:pos -> mu:nat -> a:nat -> b:nat -> nat
-let mont_mul rLen n mu a b =
+val mont_mul: pbits:pos -> rLen:nat -> n:pos -> mu:nat -> a:nat -> b:nat -> nat
+let mont_mul pbits rLen n mu a b =
   let c = a * b in
-  mont_reduction rLen n mu c
+  mont_reduction pbits rLen n mu c
 
 
 ///
@@ -209,23 +210,23 @@ let mont_mul rLen n mu a b =
 
 
 val mont_reduction_lemma_step_bound_aux:
-  rLen:nat -> n:pos -> q_i:nat{q_i < pow2 64} -> i:pos{i <= rLen} -> c:nat -> res0:nat -> Lemma
-  (requires res0 <= c + (pow2 (64 * (i - 1)) - 1) * n)
-  (ensures  res0 + n * q_i * pow2 (64 * (i - 1)) <= c + (pow2 (64 * i) - 1) * n)
+  pbits:pos -> rLen:nat -> n:pos -> q_i:nat{q_i < pow2 pbits} -> i:pos{i <= rLen} -> c:nat -> res0:nat -> Lemma
+  (requires res0 <= c + (pow2 (pbits * (i - 1)) - 1) * n)
+  (ensures  res0 + n * q_i * pow2 (pbits * (i - 1)) <= c + (pow2 (pbits * i) - 1) * n)
 
-let mont_reduction_lemma_step_bound_aux rLen n q_i i c res0 =
-  let b = pow2 (64 * i) in
-  let b1 = pow2 (64 * (i - 1)) in
+let mont_reduction_lemma_step_bound_aux pbits rLen n q_i i c res0 =
+  let b = pow2 (pbits * i) in
+  let b1 = pow2 (pbits * (i - 1)) in
 
   calc (<=) {
     res0 + n * q_i * b1;
-    (<=) { Math.Lemmas.lemma_mult_le_right b1 q_i (pow2 64 - 1) }
-    res0 + n * (pow2 64 - 1) * b1;
-    (==) { Math.Lemmas.paren_mul_right n (pow2 64 - 1) b1 }
-    res0 + n * ((pow2 64 - 1) * b1);
-    (==) { Math.Lemmas.distributivity_sub_left (pow2 64) 1 b1 }
-    res0 + n * (pow2 64 * b1 - b1);
-    (==) { Math.Lemmas.pow2_plus 64 (64 * (i - 1)) }
+    (<=) { Math.Lemmas.lemma_mult_le_right b1 q_i (pow2 pbits - 1) }
+    res0 + n * (pow2 pbits - 1) * b1;
+    (==) { Math.Lemmas.paren_mul_right n (pow2 pbits - 1) b1 }
+    res0 + n * ((pow2 pbits - 1) * b1);
+    (==) { Math.Lemmas.distributivity_sub_left (pow2 pbits) 1 b1 }
+    res0 + n * (pow2 pbits * b1 - b1);
+    (==) { Math.Lemmas.pow2_plus pbits (pbits * (i - 1)) }
     res0 + n * (b - b1);
     (==) { Math.Lemmas.distributivity_sub_right n b b1 }
     res0 + n * b - n * b1;
@@ -241,31 +242,31 @@ let mont_reduction_lemma_step_bound_aux rLen n q_i i c res0 =
 
 
 val mont_reduction_lemma_step_bound:
-  rLen:nat -> n:pos -> mu:nat -> i:pos{i <= rLen} -> c:nat -> res0:nat -> Lemma
-  (requires res0 <= c + (pow2 (64 * (i - 1)) - 1) * n)
-  (ensures  mont_reduction_f rLen n mu (i - 1) res0 <= c + (pow2 (64 * i) - 1) * n)
+  pbits:pos -> rLen:nat -> n:pos -> mu:nat -> i:pos{i <= rLen} -> c:nat -> res0:nat -> Lemma
+  (requires res0 <= c + (pow2 (pbits * (i - 1)) - 1) * n)
+  (ensures  mont_reduction_f pbits rLen n mu (i - 1) res0 <= c + (pow2 (pbits * i) - 1) * n)
 
-let mont_reduction_lemma_step_bound rLen n mu i c res0 =
-  let res = mont_reduction_f rLen n mu (i - 1) res0 in
-  let c_i = res0 / pow2 (64 * (i - 1)) % pow2 64 in
-  let q_i = mu * c_i % pow2 64 in
-  assert (res == res0 + n * q_i * pow2 (64 * (i - 1)));
-  mont_reduction_lemma_step_bound_aux rLen n q_i i c res0;
-  assert (res <= c + (pow2 (64 * i) - 1) * n)
+let mont_reduction_lemma_step_bound pbits rLen n mu i c res0 =
+  let res = mont_reduction_f pbits rLen n mu (i - 1) res0 in
+  let c_i = res0 / pow2 (pbits * (i - 1)) % pow2 pbits in
+  let q_i = mu * c_i % pow2 pbits in
+  assert (res == res0 + n * q_i * pow2 (pbits * (i - 1)));
+  mont_reduction_lemma_step_bound_aux pbits rLen n q_i i c res0;
+  assert (res <= c + (pow2 (pbits * i) - 1) * n)
 
 
 val mont_reduction_lemma_step_modr:
-  rLen:nat -> n:pos -> mu:nat -> i:pos{i <= rLen} -> c:nat -> res0:nat -> Lemma
-  (requires res0 % pow2 (64 * (i - 1)) == 0 /\ (1 + n * mu) % pow2 64 == 0)
-  (ensures  mont_reduction_f rLen n mu (i - 1) res0 % pow2 (64 * i) == 0)
+  pbits:pos -> rLen:nat -> n:pos -> mu:nat -> i:pos{i <= rLen} -> c:nat -> res0:nat -> Lemma
+  (requires res0 % pow2 (pbits * (i - 1)) == 0 /\ (1 + n * mu) % pow2 pbits == 0)
+  (ensures  mont_reduction_f pbits rLen n mu (i - 1) res0 % pow2 (pbits * i) == 0)
 
-let mont_reduction_lemma_step_modr rLen n mu i c res0 =
-  let b = pow2 (64 * i) in
-  let b1 = pow2 (64 * (i - 1)) in
+let mont_reduction_lemma_step_modr pbits rLen n mu i c res0 =
+  let b = pow2 (pbits * i) in
+  let b1 = pow2 (pbits * (i - 1)) in
 
-  let res = mont_reduction_f rLen n mu (i - 1) res0 in
-  let c_i = res0 / b1 % pow2 64 in
-  let q_i = mu * c_i % pow2 64 in
+  let res = mont_reduction_f pbits rLen n mu (i - 1) res0 in
+  let c_i = res0 / b1 % pow2 pbits in
+  let q_i = mu * c_i % pow2 pbits in
   assert (res == res0 + n * q_i * b1);
   calc (==) {
     res % b;
@@ -275,72 +276,72 @@ let mont_reduction_lemma_step_modr rLen n mu i c res0 =
     (res0 / b1 * b1 + n * q_i * b1) % b;
     (==) { Math.Lemmas.lemma_mod_plus_distr_l (res0 / b1 * b1) (n * q_i * b1) b }
     (res0 / b1 * b1 % b + n * q_i * b1) % b;
-    (==) { Math.Lemmas.pow2_multiplication_modulo_lemma_2 (res0 / b1) (64 * i) (64 * (i - 1)) }
-    (res0 / b1 % pow2 64 * b1 + n * q_i * b1) % b;
-    (==) { Math.Lemmas.distributivity_add_left (res0 / b1 % pow2 64) (n * q_i) b1 }
-    (res0 / b1 % pow2 64 + n * q_i) * b1 % b;
-    (==) { Math.Lemmas.pow2_multiplication_modulo_lemma_2 (res0 / b1 % pow2 64 + n * q_i) (64 * i) (64 * (i - 1)) }
-    (res0 / b1 % pow2 64 + n * q_i) % pow2 64 * b1;
+    (==) { Math.Lemmas.pow2_multiplication_modulo_lemma_2 (res0 / b1) (pbits * i) (pbits * (i - 1)) }
+    (res0 / b1 % pow2 pbits * b1 + n * q_i * b1) % b;
+    (==) { Math.Lemmas.distributivity_add_left (res0 / b1 % pow2 pbits) (n * q_i) b1 }
+    (res0 / b1 % pow2 pbits + n * q_i) * b1 % b;
+    (==) { Math.Lemmas.pow2_multiplication_modulo_lemma_2 (res0 / b1 % pow2 pbits + n * q_i) (pbits * i) (pbits * (i - 1)) }
+    (res0 / b1 % pow2 pbits + n * q_i) % pow2 pbits * b1;
     (==) { }
-    (c_i + n * (mu * c_i % pow2 64)) % pow2 64 * b1;
-    (==) { Math.Lemmas.lemma_mod_plus_distr_r c_i (n * (mu * c_i % pow2 64)) (pow2 64) }
-    (c_i + n * (mu * c_i % pow2 64) % pow2 64) % pow2 64 * b1;
-    (==) { Math.Lemmas.lemma_mod_mul_distr_r n (mu * c_i) (pow2 64); Math.Lemmas.paren_mul_right n mu c_i }
-    (c_i + n * mu * c_i % pow2 64) % pow2 64 * b1;
-    (==) { Math.Lemmas.lemma_mod_plus_distr_r c_i (n * mu * c_i) (pow2 64) }
-    (c_i + n * mu * c_i) % pow2 64 * b1;
+    (c_i + n * (mu * c_i % pow2 pbits)) % pow2 pbits * b1;
+    (==) { Math.Lemmas.lemma_mod_plus_distr_r c_i (n * (mu * c_i % pow2 pbits)) (pow2 pbits) }
+    (c_i + n * (mu * c_i % pow2 pbits) % pow2 pbits) % pow2 pbits * b1;
+    (==) { Math.Lemmas.lemma_mod_mul_distr_r n (mu * c_i) (pow2 pbits); Math.Lemmas.paren_mul_right n mu c_i }
+    (c_i + n * mu * c_i % pow2 pbits) % pow2 pbits * b1;
+    (==) { Math.Lemmas.lemma_mod_plus_distr_r c_i (n * mu * c_i) (pow2 pbits) }
+    (c_i + n * mu * c_i) % pow2 pbits * b1;
     (==) { Math.Lemmas.distributivity_add_left 1 (n * mu) c_i }
-    ((1 + n * mu) * c_i) % pow2 64 * b1;
-    (==) { Math.Lemmas.lemma_mod_mul_distr_l (1 + n * mu) c_i (pow2 64) }
-    ((1 + n * mu) % pow2 64 * c_i) % pow2 64 * b1;
-    (==) { assert ((1 + n * mu) % pow2 64 == 0) }
+    ((1 + n * mu) * c_i) % pow2 pbits * b1;
+    (==) { Math.Lemmas.lemma_mod_mul_distr_l (1 + n * mu) c_i (pow2 pbits) }
+    ((1 + n * mu) % pow2 pbits * c_i) % pow2 pbits * b1;
+    (==) { assert ((1 + n * mu) % pow2 pbits == 0) }
     0;
   };
   assert (res % b == 0)
 
 
 val mont_reduction_lemma_step_modn:
-  rLen:nat -> n:pos -> mu:nat -> i:pos{i <= rLen} -> c:nat -> res0:nat -> Lemma
+  pbits:pos -> rLen:nat -> n:pos -> mu:nat -> i:pos{i <= rLen} -> c:nat -> res0:nat -> Lemma
   (requires res0 % n == c % n)
-  (ensures  mont_reduction_f rLen n mu (i - 1) res0 % n == c % n)
+  (ensures  mont_reduction_f pbits rLen n mu (i - 1) res0 % n == c % n)
 
-let mont_reduction_lemma_step_modn rLen n mu i c res0 =
-  let res = mont_reduction_f rLen n mu (i - 1) res0 in
-  let c_i = res0 / pow2 (64 * (i - 1)) % pow2 64 in
-  let q_i = mu * c_i % pow2 64 in
-  assert (res == res0 + n * q_i * pow2 (64 * (i - 1)));
-  Math.Lemmas.paren_mul_right n q_i (pow2 (64 * (i - 1)));
-  Math.Lemmas.modulo_addition_lemma res0 n (q_i * pow2 (64 * (i - 1)))
+let mont_reduction_lemma_step_modn pbits rLen n mu i c res0 =
+  let res = mont_reduction_f pbits rLen n mu (i - 1) res0 in
+  let c_i = res0 / pow2 (pbits * (i - 1)) % pow2 pbits in
+  let q_i = mu * c_i % pow2 pbits in
+  assert (res == res0 + n * q_i * pow2 (pbits * (i - 1)));
+  Math.Lemmas.paren_mul_right n q_i (pow2 (pbits * (i - 1)));
+  Math.Lemmas.modulo_addition_lemma res0 n (q_i * pow2 (pbits * (i - 1)))
 
 
 val mont_reduction_lemma_step:
-  rLen:nat -> n:pos -> mu:nat -> i:pos{i <= rLen} -> c:nat -> res0:nat -> Lemma
+  pbits:pos -> rLen:nat -> n:pos -> mu:nat -> i:pos{i <= rLen} -> c:nat -> res0:nat -> Lemma
   (requires
-    res0 % n == c % n /\ res0 % pow2 (64 * (i - 1)) == 0 /\
-    res0 <= c + (pow2 (64 * (i - 1)) - 1) * n /\ (1 + n * mu) % pow2 64 == 0)
-  (ensures  (let res = mont_reduction_f rLen n mu (i - 1) res0 in
-    res % n == c % n /\ res % pow2 (64 * i) == 0 /\ res <= c + (pow2 (64 * i) - 1) * n))
+    res0 % n == c % n /\ res0 % pow2 (pbits * (i - 1)) == 0 /\
+    res0 <= c + (pow2 (pbits * (i - 1)) - 1) * n /\ (1 + n * mu) % pow2 pbits == 0)
+  (ensures  (let res = mont_reduction_f pbits rLen n mu (i - 1) res0 in
+    res % n == c % n /\ res % pow2 (pbits * i) == 0 /\ res <= c + (pow2 (pbits * i) - 1) * n))
 
-let mont_reduction_lemma_step rLen n mu i c res0 =
-  mont_reduction_lemma_step_bound rLen n mu i c res0;
-  mont_reduction_lemma_step_modr rLen n mu i c res0;
-  mont_reduction_lemma_step_modn rLen n mu i c res0
+let mont_reduction_lemma_step pbits rLen n mu i c res0 =
+  mont_reduction_lemma_step_bound pbits rLen n mu i c res0;
+  mont_reduction_lemma_step_modr pbits rLen n mu i c res0;
+  mont_reduction_lemma_step_modn pbits rLen n mu i c res0
 
 
-val mont_reduction_loop_lemma: rLen:nat -> n:pos -> mu:nat -> i:nat{i <= rLen} -> c:nat -> Lemma
-  (requires (1 + n * mu) % pow2 64 == 0)
-  (ensures  (let res = repeati i (mont_reduction_f rLen n mu) c in
-    res % n == c % n /\ res % pow2 (64 * i) == 0 /\ res <= c + (pow2 (64 * i) - 1) * n))
+val mont_reduction_loop_lemma: pbits:pos -> rLen:nat -> n:pos -> mu:nat -> i:nat{i <= rLen} -> c:nat -> Lemma
+  (requires (1 + n * mu) % pow2 pbits == 0)
+  (ensures  (let res = repeati i (mont_reduction_f pbits rLen n mu) c in
+    res % n == c % n /\ res % pow2 (pbits * i) == 0 /\ res <= c + (pow2 (pbits * i) - 1) * n))
 
-let rec mont_reduction_loop_lemma rLen n mu i c =
-  let res : nat = repeati i (mont_reduction_f rLen n mu) c in
+let rec mont_reduction_loop_lemma pbits rLen n mu i c =
+  let res : nat = repeati i (mont_reduction_f pbits rLen n mu) c in
   if i = 0 then
-    eq_repeati0 i (mont_reduction_f rLen n mu) c
+    eq_repeati0 i (mont_reduction_f pbits rLen n mu) c
   else begin
-    unfold_repeati i (mont_reduction_f rLen n mu) c (i - 1);
-    let res0 : nat = repeati (i - 1) (mont_reduction_f rLen n mu) c in
-    mont_reduction_loop_lemma rLen n mu (i - 1) c;
-    mont_reduction_lemma_step rLen n mu i c res0 end
+    unfold_repeati i (mont_reduction_f pbits rLen n mu) c (i - 1);
+    let res0 : nat = repeati (i - 1) (mont_reduction_f pbits rLen n mu) c in
+    mont_reduction_loop_lemma pbits rLen n mu (i - 1) c;
+    mont_reduction_lemma_step pbits rLen n mu i c res0 end
 
 
 val lemma_fits_aux: c:nat -> r:pos -> n:pos -> Lemma
@@ -353,14 +354,15 @@ let lemma_fits_aux c r n =
   Math.Lemmas.lemma_div_le (c - n) c r
 
 
-val mont_mult_lemma_fits_aux: rLen:nat -> n:pos -> mu:nat -> c:nat -> Lemma
-  (requires (1 + n * mu) % pow2 64 == 0 /\ n < pow2 (64 * rLen) /\ c < n * n)
-  (ensures  (let res : nat = repeati rLen (mont_reduction_f rLen n mu) c in res / pow2 (64 * rLen) < 2 * n))
+val mont_mult_lemma_fits_aux: pbits:pos -> rLen:nat -> n:pos -> mu:nat -> c:nat -> Lemma
+  (requires (1 + n * mu) % pow2 pbits == 0 /\ n < pow2 (pbits * rLen) /\ c < n * n)
+  (ensures  (let res : nat = repeati rLen (mont_reduction_f pbits rLen n mu) c in
+    res / pow2 (pbits * rLen) < 2 * n))
 
-let mont_mult_lemma_fits_aux rLen n mu c =
-  let r = pow2 (64 * rLen) in
-  let res : nat = repeati rLen (mont_reduction_f rLen n mu) c in
-  mont_reduction_loop_lemma rLen n mu rLen c;
+let mont_mult_lemma_fits_aux pbits rLen n mu c =
+  let r = pow2 (pbits * rLen) in
+  let res : nat = repeati rLen (mont_reduction_f pbits rLen n mu) c in
+  mont_reduction_loop_lemma pbits rLen n mu rLen c;
   assert (res <= c + (r - 1) * n /\ res % r == 0);
   Math.Lemmas.lemma_div_le res (c + (r - 1) * n) r;
   assert (res / r <= (c + (r - 1) * n) / r);
@@ -376,29 +378,29 @@ let mont_mult_lemma_fits_aux rLen n mu c =
   assert (res / r < 2 * n)
 
 
-val mont_mult_lemma_fits: rLen:nat -> n:pos -> mu:nat -> c:nat -> Lemma
-  (requires (1 + n * mu) % pow2 64 == 0 /\ n < pow2 (64 * rLen) /\ c < n * n)
-  (ensures mont_reduction rLen n mu c < n)
+val mont_mult_lemma_fits: pbits:pos -> rLen:nat -> n:pos -> mu:nat -> c:nat -> Lemma
+  (requires (1 + n * mu) % pow2 pbits == 0 /\ n < pow2 (pbits * rLen) /\ c < n * n)
+  (ensures mont_reduction pbits rLen n mu c < n)
 
-let mont_mult_lemma_fits rLen n mu c =
-  let r = pow2 (64 * rLen) in
-  let res : nat = repeati rLen (mont_reduction_f rLen n mu) c in
+let mont_mult_lemma_fits pbits rLen n mu c =
+  let r = pow2 (pbits * rLen) in
+  let res : nat = repeati rLen (mont_reduction_f pbits rLen n mu) c in
   let res = res / r in
-  mont_mult_lemma_fits_aux rLen n mu c;
+  mont_mult_lemma_fits_aux pbits rLen n mu c;
   let res1 = if res < n then res else res - n in
   assert (res1 < n)
 
 
-val mont_reduction_lemma: rLen:nat -> n:pos -> d:int-> mu:nat -> c:nat -> Lemma
+val mont_reduction_lemma: pbits:pos -> rLen:nat -> n:pos -> d:int-> mu:nat -> c:nat -> Lemma
   (requires
-    (1 + n * mu) % pow2 64 == 0 /\ pow2 (64 * rLen) * d % n == 1 /\
-    n < pow2 (64 * rLen) /\ c < n * n)
-  (ensures  mont_reduction rLen n mu c == c * d % n)
+    (1 + n * mu) % pow2 pbits == 0 /\ pow2 (pbits * rLen) * d % n == 1 /\
+    n < pow2 (pbits * rLen) /\ c < n * n)
+  (ensures  mont_reduction pbits rLen n mu c == c * d % n)
 
-let mont_reduction_lemma rLen n d mu c =
-  let r = pow2 (64 * rLen) in
-  let res : nat = repeati rLen (mont_reduction_f rLen n mu) c in
-  mont_reduction_loop_lemma rLen n mu rLen c;
+let mont_reduction_lemma pbits rLen n d mu c =
+  let r = pow2 (pbits * rLen) in
+  let res : nat = repeati rLen (mont_reduction_f pbits rLen n mu) c in
+  mont_reduction_loop_lemma pbits rLen n mu rLen c;
   assert (res % n == c % n /\ res % r == 0 /\ res <= c + (r - 1) * n);
   calc (==) {
     res / r % n;
@@ -423,7 +425,7 @@ let mont_reduction_lemma rLen n d mu c =
   let res2 = if res1 < n then res1 else res1 - n in
   Math.Lemmas.lemma_mod_sub res1 n 1;
   assert (res2 % n == res1 % n);
-  mont_mult_lemma_fits rLen n mu c;
+  mont_mult_lemma_fits pbits rLen n mu c;
   Math.Lemmas.small_mod res2 n
 
 ///
@@ -446,25 +448,27 @@ let lemma_mod_mul_distr3 a b c n =
   }
 
 
-val to_mont_lemma: rLen:nat -> n:pos -> d:int-> mu:nat -> a:nat -> Lemma
+val to_mont_lemma: pbits:pos -> rLen:nat -> n:pos -> d:int-> mu:nat -> a:nat -> Lemma
   (requires
-    (1 + n * mu) % pow2 64 == 0 /\ pow2 (64 * rLen) * d % n == 1 /\
-    n < pow2 (64 * rLen) /\ a < n)
-  (ensures  to_mont rLen n mu a == a * pow2 (64 * rLen) % n)
+    (1 + n * mu) % pow2 pbits == 0 /\ pow2 (pbits * rLen) * d % n == 1 /\
+    n < pow2 (pbits * rLen) /\ a < n)
+  (ensures  to_mont pbits rLen n mu a == a * pow2 (pbits * rLen) % n)
 
-let to_mont_lemma rLen n d mu a =
-  let r = pow2 (64 * rLen) in
-  let r2 = pow2 (128 * rLen) % n in
+let to_mont_lemma pbits rLen n d mu a =
+  let r = pow2 (pbits * rLen) in
+  let r2 = pow2 (2 * pbits * rLen) % n in
   let c = a * r2 in
-  let aM = to_mont rLen n mu a in
-  assert (aM == mont_reduction rLen n mu c);
-  mont_reduction_lemma rLen n d mu c;
+  let aM = to_mont pbits rLen n mu a in
+  assert (aM == mont_reduction pbits rLen n mu c);
+  Math.Lemmas.lemma_mult_lt_sqr a r2 n;
+  mont_reduction_lemma pbits rLen n d mu c;
   assert (aM == c * d % n);
   calc (==) {
     c * d % n;
     (==) { }
     a * r2 * d % n;
-    (==) { Math.Lemmas.pow2_plus (64 * rLen) (64 * rLen) }
+    (==) { Math.Lemmas.paren_mul_right 2 pbits rLen;
+           Math.Lemmas.pow2_plus (pbits * rLen) (pbits * rLen) }
     a * (r * r % n) * d % n;
     (==) { lemma_mod_mul_distr3 a (r * r) d n }
     a * (r * r) * d % n;
@@ -483,14 +487,14 @@ let to_mont_lemma rLen n d mu a =
 ///  Lemma (from_mont rLen n mu aM == aM * d % n)
 ///
 
-val from_mont_lemma: rLen:nat -> n:pos -> d:int -> mu:nat -> aM:nat -> Lemma
+val from_mont_lemma: pbits:pos -> rLen:nat -> n:pos -> d:int -> mu:nat -> aM:nat -> Lemma
   (requires
-    (1 + n * mu) % pow2 64 == 0 /\ pow2 (64 * rLen) * d % n == 1 /\
-    n < pow2 (64 * rLen) /\ aM < n)
-  (ensures  from_mont rLen n mu aM == aM * d % n)
+    (1 + n * mu) % pow2 pbits == 0 /\ pow2 (pbits * rLen) * d % n == 1 /\
+    n < pow2 (pbits * rLen) /\ aM < n)
+  (ensures  from_mont pbits rLen n mu aM == aM * d % n)
 
-let from_mont_lemma rLen n d mu aM =
-  mont_reduction_lemma rLen n d mu aM
+let from_mont_lemma pbits rLen n d mu aM =
+  mont_reduction_lemma pbits rLen n d mu aM
 
 ///
 ///  Properties of Montgomery arithmetic
