code/bignum/Hacl.Spec.Bignum.ModInvLimb.fsti
@@ -1,0 +1,16 @@
+module Hacl.Spec.Bignum.ModInvLimb
+
+open FStar.Mul
+
+open Lib.IntTypes
+open Hacl.Spec.Bignum.Definitions
+
+#reset-options "--z3rlimit 50 --fuel 0 --ifuel 0"
+
+(** Precomputed constant for Montgomery arithmetic *)
+
+val mod_inv_limb: #t:limb_t -> n0:limb t -> limb t
+
+val mod_inv_limb_lemma: #t:limb_t -> n0:limb t -> Lemma
+  (requires v n0 % 2 == 1)
+  (ensures (1 + v n0 * v (mod_inv_limb n0)) % pow2 (bits t) == 0)
