code/bignum/Hacl.Spec.Bignum.Montgomery.fsti
@@ -14,140 +14,150 @@ module M = Hacl.Spec.Montgomery.Lemmas
 ///  check a modulus for Montgomery arithmetic
 ///
 
-val check_modulus: #nLen:size_pos{128 * nLen <= max_size_t} -> n:lbignum nLen ->
-  res:uint64{v res == (if (bn_v n % 2 = 1 && 1 < bn_v n) then v (ones U64 SEC) else v (zeros U64 SEC))}
+val check_modulus: #t:limb_t -> #nLen:size_pos{2 * bits t * nLen <= max_size_t} -> n:lbignum t nLen ->
+  res:limb t{v res == (if (bn_v n % 2 = 1 && 1 < bn_v n) then v (ones t SEC) else v (zeros t SEC))}
 
 ///
 ///  Precomputed constants for Montgomery arithmetic
 ///
 
-val precomp_r2_mod_n: #nLen:size_pos{128 * nLen <= max_size_t} -> n:lbignum nLen -> lbignum nLen
+val precomp_r2_mod_n: #t:limb_t -> #nLen:size_pos{2 * bits t * nLen <= max_size_t} -> n:lbignum t nLen -> lbignum t nLen
 
-val precomp_r2_mod_n_lemma: #nLen:size_pos -> n:lbignum nLen -> Lemma
-  (requires 1 < bn_v n /\ bn_v n % 2 = 1 /\ 128 * nLen <= max_size_t)
-  (ensures  bn_v (precomp_r2_mod_n n) == pow2 (128 * nLen) % bn_v n)
+val precomp_r2_mod_n_lemma: #t:limb_t -> #nLen:size_pos -> n:lbignum t nLen -> Lemma
+  (requires 1 < bn_v n /\ bn_v n % 2 = 1 /\ 2 * bits t * nLen <= max_size_t)
+  (ensures  bn_v (precomp_r2_mod_n n) == pow2 (2 * bits t * nLen) % bn_v n)
 
 ///
 ///  Conversion functions to/from the Montgomery domen and the Montgomery reduction
 ///
 
 val mont_reduction:
-    #nLen:size_pos{nLen + nLen <= max_size_t}
-  -> n:lbignum nLen
-  -> mu:uint64
-  -> c:lbignum (nLen + nLen) ->
-  lbignum nLen
+    #t:limb_t
+  -> #nLen:size_pos{nLen + nLen <= max_size_t}
+  -> n:lbignum t nLen
+  -> mu:limb t
+  -> c:lbignum t (nLen + nLen) ->
+  lbignum t nLen
 
 
 val to_mont:
-    #nLen:size_pos{nLen + nLen <= max_size_t}
-  -> n:lbignum nLen
-  -> mu:uint64
-  -> r2:lbignum nLen
-  -> a:lbignum nLen ->
-  lbignum nLen
+    #t:limb_t
+  -> #nLen:size_pos{nLen + nLen <= max_size_t}
+  -> n:lbignum t nLen
+  -> mu:limb t
+  -> r2:lbignum t nLen
+  -> a:lbignum t nLen ->
+  lbignum t nLen
 
 
 val from_mont:
-    #nLen:size_pos{nLen + nLen <= max_size_t}
-  -> n:lbignum nLen
-  -> mu:uint64
-  -> aM:lbignum nLen ->
-  lbignum nLen
+    #t:limb_t
+  -> #nLen:size_pos{nLen + nLen <= max_size_t}
+  -> n:lbignum t nLen
+  -> mu:limb t
+  -> aM:lbignum t nLen ->
+  lbignum t nLen
 
 
 val mont_mul:
-    #nLen:size_pos{nLen + nLen <= max_size_t}
-  -> n:lbignum nLen
-  -> mu:uint64
-  -> aM:lbignum nLen
-  -> bM:lbignum nLen ->
-  lbignum nLen
+    #t:limb_t
+  -> #nLen:size_pos{nLen + nLen <= max_size_t}
+  -> n:lbignum t nLen
+  -> mu:limb t
+  -> aM:lbignum t nLen
+  -> bM:lbignum t nLen ->
+  lbignum t nLen
 
 
 val mont_sqr:
-    #nLen:size_pos{nLen + nLen <= max_size_t}
-  -> n:lbignum nLen
-  -> mu:uint64
-  -> aM:lbignum nLen ->
-  lbignum nLen
+    #t:limb_t
+  -> #nLen:size_pos{nLen + nLen <= max_size_t}
+  -> n:lbignum t nLen
+  -> mu:limb t
+  -> aM:lbignum t nLen ->
+  lbignum t nLen
 
 ///
 ///  Lemmas
 ///
 
 val mont_reduction_lemma:
-    #nLen:size_pos{nLen + nLen <= max_size_t}
-  -> n:lbignum nLen
-  -> mu:uint64
-  -> c:lbignum (nLen + nLen) -> Lemma
+    #t:limb_t
+  -> #nLen:size_pos{nLen + nLen <= max_size_t}
+  -> n:lbignum t nLen
+  -> mu:limb t
+  -> c:lbignum t (nLen + nLen) -> Lemma
   (requires
-    (1 + (bn_v n % pow2 64) * v mu) % pow2 64 == 0 /\
+    (1 + (bn_v n % pow2 (bits t)) * v mu) % pow2 (bits t) == 0 /\
     bn_v n % 2 = 1 /\ 1 < bn_v n /\
     bn_v c < bn_v n * bn_v n)
   (ensures
-    (let res = bn_v (mont_reduction #nLen n mu c) in
-    res == M.mont_reduction nLen (bn_v n) (v mu) (bn_v c) /\
+    (let res = bn_v (mont_reduction n mu c) in
+    res == M.mont_reduction (bits t) nLen (bn_v n) (v mu) (bn_v c) /\
     res < bn_v n))
 
 
 val to_mont_lemma:
-    #nLen:size_pos{nLen + nLen <= max_size_t}
-  -> n:lbignum nLen
-  -> mu:uint64
-  -> r2:lbignum nLen
-  -> a:lbignum nLen -> Lemma
+    #t:limb_t
+  -> #nLen:size_pos{nLen + nLen <= max_size_t}
+  -> n:lbignum t nLen
+  -> mu:limb t
+  -> r2:lbignum t nLen
+  -> a:lbignum t nLen -> Lemma
   (requires
-    (1 + (bn_v n % pow2 64) * v mu) % pow2 64 == 0 /\
+    (1 + (bn_v n % pow2 (bits t)) * v mu) % pow2 (bits t) == 0 /\
     bn_v n % 2 = 1 /\ 1 < bn_v n /\
-    bn_v a < bn_v n /\ bn_v r2 == pow2 (128 * nLen) % bn_v n)
+    bn_v a < bn_v n /\ bn_v r2 == pow2 (2 * bits t * nLen) % bn_v n)
   (ensures
-   (let aM = bn_v (to_mont #nLen n mu r2 a) in
-    aM == M.to_mont nLen (bn_v n) (v mu) (bn_v a) /\
+   (let aM = bn_v (to_mont n mu r2 a) in
+    aM == M.to_mont (bits t) nLen (bn_v n) (v mu) (bn_v a) /\
     aM < bn_v n))
 
 
 val from_mont_lemma:
-    #nLen:size_pos{nLen + nLen <= max_size_t}
-  -> n:lbignum nLen
-  -> mu:uint64
-  -> aM:lbignum nLen -> Lemma
+    #t:limb_t
+  -> #nLen:size_pos{nLen + nLen <= max_size_t}
+  -> n:lbignum t nLen
+  -> mu:limb t
+  -> aM:lbignum t nLen -> Lemma
   (requires
-    (1 + (bn_v n % pow2 64) * v mu) % pow2 64 == 0 /\
+    (1 + (bn_v n % pow2 (bits t)) * v mu) % pow2 (bits t) == 0 /\
     bn_v n % 2 = 1 /\ 1 < bn_v n /\
     bn_v aM < bn_v n)
   (ensures
-   (let a = bn_v (from_mont #nLen n mu aM) in
-    a == M.from_mont nLen (bn_v n) (v mu) (bn_v aM) /\
+   (let a = bn_v (from_mont n mu aM) in
+    a == M.from_mont (bits t) nLen (bn_v n) (v mu) (bn_v aM) /\
     a < bn_v n))
 
 
 val mont_mul_lemma:
-    #nLen:size_pos{nLen + nLen <= max_size_t}
-  -> n:lbignum nLen
-  -> mu:uint64
-  -> aM:lbignum nLen
-  -> bM:lbignum nLen -> Lemma
+    #t:limb_t
+  -> #nLen:size_pos{nLen + nLen <= max_size_t}
+  -> n:lbignum t nLen
+  -> mu:limb t
+  -> aM:lbignum t nLen
+  -> bM:lbignum t nLen -> Lemma
   (requires
-    (1 + (bn_v n % pow2 64) * v mu) % pow2 64 == 0 /\
+    (1 + (bn_v n % pow2 (bits t)) * v mu) % pow2 (bits t) == 0 /\
     bn_v n % 2 = 1 /\ 1 < bn_v n /\
     bn_v aM < bn_v n /\ bn_v bM < bn_v n)
   (ensures
-    (let res = bn_v (mont_mul #nLen n mu aM bM) in
-    res == M.mont_mul nLen (bn_v n) (v mu) (bn_v aM) (bn_v bM) /\
+    (let res = bn_v (mont_mul n mu aM bM) in
+    res == M.mont_mul (bits t) nLen (bn_v n) (v mu) (bn_v aM) (bn_v bM) /\
     res < bn_v n))
 
 
 val mont_sqr_lemma:
-    #nLen:size_pos{nLen + nLen <= max_size_t}
-  -> n:lbignum nLen
-  -> mu:uint64
-  -> aM:lbignum nLen -> Lemma
+    #t:limb_t
+  -> #nLen:size_pos{nLen + nLen <= max_size_t}
+  -> n:lbignum t nLen
+  -> mu:limb t
+  -> aM:lbignum t nLen -> Lemma
   (requires
-    (1 + (bn_v n % pow2 64) * v mu) % pow2 64 == 0 /\
+    (1 + (bn_v n % pow2 (bits t)) * v mu) % pow2 (bits t) == 0 /\
     bn_v n % 2 = 1 /\ 1 < bn_v n /\
     bn_v aM < bn_v n)
   (ensures
-    (let res = bn_v (mont_sqr #nLen n mu aM) in
-    res == M.mont_mul nLen (bn_v n) (v mu) (bn_v aM) (bn_v aM) /\
+    (let res = bn_v (mont_sqr n mu aM) in
+    res == M.mont_mul (bits t) nLen (bn_v n) (v mu) (bn_v aM) (bn_v aM) /\
     res < bn_v n))
